@prefix pt: <http://parliament.uk/ontologies/time-period/> . 
@prefix xsd: <http://www.w3.org/2001/XMLSchema#> . 
@prefix rdf: <http://www.w3.org/1999/02/22-rdf-syntax-ns#> .
@prefix dcterms: <http://purl.org/dc/terms/> .
@prefix owl:     <http://www.w3.org/2002/07/owl#> .
@prefix rdfs:    <http://www.w3.org/2000/01/rdf-schema#> .

<http://parliament.uk/ontologies/time-point/> 
    rdf:type owl:Ontology ;
    dcterms:title "Time period ontology"@en ;
    dcterms:created "2017-03-09"^^xsd:date ;
	dcterms:rights "Open Parliament Licence v3.0"@en ;
    dcterms:description "Ontology to describe high level time periods for UK Parliament"@en .


#######  Classes #####

pt:Agent rdf:type owl:Class ;
	rdfs:label "Agent"@en ;
	rdfs:comment "An agent. The superset of all people and all groups of people."@en ;
	rdfs:isDefinedBy <http://parliament.uk/ontologies/time-period/> .

pt:Event rdf:type owl:Class ;
	rdfs:label "Event"@en ;
	rdfs:comment "A discrete event involving agents, locations and / or outputs. Events frequently initiate changes between time periods. Examples might be: State Opening, coronation, abdication, general election, prorogation, dissolution, recall."@en ;
	rdfs:isDefinedBy <http://parliament.uk/ontologies/time-period/> .

pt:TimePeriod rdf:type owl:Class ;
	rdfs:label "TimePeriod"@en ;
	rdfs:comment "An identifiable and named period of time. An interval."@en ;
	rdfs:isDefinedBy <http://parliament.uk/ontologies/time-period/> .

pt:GovernmentAdministrationPeriod rdf:type owl:Class ;
	rdfs:subClassOf pt:TimePeriod ;
	rdfs:label "GovernmentAdministrationPeriod"@en ;
	rdfs:comment "A period of a single government under a single Prime Minister bounded by parliaments / general elections. e.g. Thatcher administration 1979-1983, Thatcher administration 1983-1987, Thatcher administration 1987-1990."@en ;
	rdfs:isDefinedBy <http://parliament.uk/ontologies/time-period/> .

pt:PremiershipPeriod rdf:type owl:Class ;
	rdfs:subClassOf pt:TimePeriod ;
	rdfs:label "PremiershipPeriod"@en ;
	rdfs:comment "A grouping of periods of government under a single Prime Minister not bounded by parliaments / general elections. e.g. Thatcher administration 1979-1990."@en ;
	rdfs:isDefinedBy <http://parliament.uk/ontologies/time-period/> .

pt:Reign rdf:type owl:Class ;
	rdfs:subClassOf pt:TimePeriod ;
	rdfs:label "Reign"@en ;
	rdfs:comment "The period under a monarch."@en ;
	rdfs:isDefinedBy <http://parliament.uk/ontologies/time-period/> .

pt:ParliamentPeriod rdf:type owl:Class ;
	rdfs:subClassOf pt:TimePeriod ;
	rdfs:label "ParliamentPeriod"@en ;
	rdfs:comment "The period of a single Parliament between its first assembly after a general election and its dissolution. A parliament period contains session and prorogation periods. These run contiguously within a parliament period. In other words, during a parliament period, Parliament is either in session or prorogued. A Parliament begins on the date named in the proclamation which is now issued after a dissolution (until 2015 the dissolution proclamation also named the date for Parliament to reassemble). The start date of a Parliament may be changed by subsequent proclamations. A Parliament ends at the next dissolution, the date of which is determined by the Fixed Term Parliament Act 2011 or is named in a proclamation after Parliament has voted for an early general election (before 2015 the date of dissolution was indeterminate and fixed by proclamation). Parliament periods are the same across both Houses. Parliaments are numbered in sequence from the first Parliament of the United Kingdom beginning with 1801. As of April 2018, the current Parliament is the 57th."@en ;
	rdfs:isDefinedBy <http://parliament.uk/ontologies/time-period/> .
	
pt:DissolutionPeriod rdf:type owl:Class ;
	rdfs:subClassOf pt:TimePeriod ;
	rdfs:label "DissolutionPeriod"@en ;
	rdfs:comment "The period between parliament periods. Parliament is dissolved. During this time no parliamentary business can take place. From the point of dissolution until the general election there are no Members of the House of Commons. Note that Members of the House of Commons are considered Members on election even though Parliament is dissolved. Members of the House of Lords retain their positions during dissolution. Dissolution periods are the same across both Houses."@en ;
	rdfs:isDefinedBy <http://parliament.uk/ontologies/time-period/> .
	
pt:PreElectionDissolutionPeriod rdf:type owl:Class ;
	rdfs:subClassOf pt:TimePeriod ;
	rdfs:label "PreElectionDissolutionPeriod"@en ;
	rdfs:comment "The period between the end of a parliament period and the results of all constituency elections being announced. During this time there are no Members of the House of Commons."@en ;
	rdfs:isDefinedBy <http://parliament.uk/ontologies/time-period/> .
	
pt:PostElectionDissolutionPeriod rdf:type owl:Class ;
	rdfs:subClassOf pt:TimePeriod ;
	rdfs:label "PostElectionDissolutionPeriod"@en ;
	rdfs:comment "The period between the results of all constituency elections being announced and the next parliament period. During this period, successful candidates are considered to be Members even though Parliament is dissolved."@en ;
	rdfs:isDefinedBy <http://parliament.uk/ontologies/time-period/> .

pt:Session rdf:type owl:Class ;
	rdfs:subClassOf pt:TimePeriod ;
	rdfs:label "Session"@en ;
	rdfs:comment "The period during which Parliament is convened. The first session of a parliament begins on the same day as the parliament period: this date is given in the dissolution proclamation at the end of the previous parliament. The session ends on the day set in a subsequent prorogation proclamation. Subsequent sessions within the parliament period begin and end on dates set in subsequent prorogation proclamations. The final session of a parliament ends either with prorogation followed by dissolution or with dissolution. Session periods are the same for both Houses."@en ;
	rdfs:isDefinedBy <http://parliament.uk/ontologies/time-period/> .
	
pt:ProrogationPeriod rdf:type owl:Class ;
	rdfs:subClassOf pt:TimePeriod ;
	rdfs:label "ProrogationPeriod"@en ;
	rdfs:comment "The period during which Parliament is inactive between prorogation and the start of the subsequent session or dissolution. During this time there are still Members but all parliamentary business stops. Prorogation periods are the same across both Houses."@en ;
	rdfs:isDefinedBy <http://parliament.uk/ontologies/time-period/> .
	
pt:Term rdf:type owl:Class ;
	rdfs:subClassOf pt:TimePeriod ;
	rdfs:label "Term"@en ;
	rdfs:comment "The period between recess periods during which Parliament is active, and may be sitting. This period does not have an official name. Term periods are not necessarily the same across both Houses."@en ;
	rdfs:isDefinedBy <http://parliament.uk/ontologies/time-period/> .

pt:Recess rdf:type owl:Class ;
	rdfs:subClassOf pt:TimePeriod ;
	rdfs:label "Recess"@en ;
	rdfs:comment "A period during a session when one or both Houses have adjourned to a day other than the next usual sitting day, which may last between a few days and several weeks. Officially, a recess is the period when Parliament is prorogued, but it is now used to indicate what are officially known as periodic adjournments (which would normally be called holidays). A periodic adjournment may be ended by a prorogation or a dissolution."@en ;
	rdfs:isDefinedBy <http://parliament.uk/ontologies/time-period/> .

pt:SittingDay rdf:type owl:Class ;
	rdfs:subClassOf pt:TimePeriod ;
	rdfs:label "SittingDay"@en ;
	rdfs:comment "A day on which a House is sitting. Sitting days are not the same across both Houses. A sitting day may continue after midnight and therefore cross more than one calendar day, but it is known by the day on which it started."@en ;
	rdfs:isDefinedBy <http://parliament.uk/ontologies/time-period/> .
	
pt:TablingDay rdf:type owl:Class ;
	rdfs:subClassOf pt:TimePeriod ;
	rdfs:label "TablingDay"@en ;
	rdfs:comment "A day on which it is possible for a Member of a House to table a question. In the House of Commons questions can only be tabled on sitting days. In the House of Lords questions can also be tabled on selected recess days."@en ;
	rdfs:isDefinedBy <http://parliament.uk/ontologies/time-period/> .
	
pt:StatutoryDay rdf:type owl:Class ;
	rdfs:subClassOf pt:TimePeriod ;
	rdfs:label "StatutoryDay"@en ;
	rdfs:comment "There is a defined period of time during which Members of either House can object to negative and made affirmative statutory instruments. Only certain calendar days are included when calculating this period. The total number and nature of days on which a Member can object are defined by statute and differ across parliamentary procedure. These statutory days comprise consecutive days including weekends, excluding any days during which Parliament is dissolved, or prorogued, or any period during which both Houses are adjourned for more than four days. Differences in sitting days between Houses are not taken into account, unless the instrument is laid into the House of Commons only. In this case the calculation is based on Commons sitting days and short adjournments. On the day on which a negative statutory instrument is laid, a forty day time period commences during which it is possible for Members to 'pray' against (table a motion objecting to) the instrument. This forty day period is defined by the Statutory Instruments Act 1946. For made affirmative statutory instruments the time limit is set out in the enabling Act, rather than in the Statutory Instruments Act 1946. It is typically 28 or 40 days. The time period commences on the day the instrument is made, rather than laid. The enabling Act stipulates which days are counted towards the time limit, and typically follows the logic previously described."@en ;
	rdfs:isDefinedBy <http://parliament.uk/ontologies/time-period/> .
	
pt:PrintingDay rdf:type owl:Class ;
	rdfs:subClassOf pt:TimePeriod ;
	rdfs:label "PrintingDay"@en ;
	rdfs:comment "In the House of Commons, a printing day is a non-sitting day during an adjournment (not including a non-sitting Friday) on which any parliamentary questions or amendments to Bills tabled since the last sitting day are published. The parliamentary questions so published are not officially tabled until the next sitting day, but under House of Commons Standing Order No. 64 (retrieved at 17/04/2018), amendments to Bills received before 16h30 on the last business day of the period are treated as if that day were a sitting day."@en ;
	rdfs:isDefinedBy <http://parliament.uk/ontologies/time-period/> .

pt:House rdf:type owl:Class ;
	rdfs:subClassOf pt:TimePeriod ;
	rdfs:label "House"@en ;
	rdfs:comment "A parliamentary House e.g. the House of Lords."@en ;
	rdfs:isDefinedBy <http://parliament.uk/ontologies/time-period/> .


				
#######  Object properties ##### 

pt:initiatesEvent rdf:type owl:ObjectProperty ;
	rdfs:label "initiatesEvent"@en ;
	rdfs:comment "Relates an agent to an event they initiate."@en ;
	rdfs:domain pt:Agent ;
	rdfs:range pt:Event ;
	rdfs:isDefinedBy <http://parliament.uk/ontologies/time-period/> .
	
pt:initiatesTimePeriod rdf:type owl:ObjectProperty ;
	rdfs:label "initiatesTimePeriod"@en ;
	rdfs:comment "Relates an event to a time period it initiates."@en ;
	rdfs:domain pt:Event ;
	rdfs:range pt:TimePeriod ;
	rdfs:isDefinedBy <http://parliament.uk/ontologies/time-period/> .
	
pt:containedIn rdf:type owl:ObjectProperty ;
	rdfs:label "containedIn"@en ;
	rdfs:comment "Relates an event to a time period it's contained in."@en ;
	rdfs:domain pt:Event ;
	rdfs:range pt:TimePeriod ;
	rdfs:isDefinedBy <http://parliament.uk/ontologies/time-period/> .
	
pt:partOfPremiershipPeriod rdf:type owl:ObjectProperty ;
	rdfs:label "partOfPremiershipPeriod"@en ;
	rdfs:comment "Relates a government administration period to a premiership period. e.g. allows for grouping of 3 Thatcher administrations into one 'premiership'."@en ;
	rdfs:domain pt:GovernmentAdministrationPeriod ;
	rdfs:range pt:PremiershipPeriod ;
	rdfs:isDefinedBy <http://parliament.uk/ontologies/time-period/> .
	
pt:hasSession rdf:type owl:ObjectProperty ;
	rdfs:label "hasSession"@en ;
	rdfs:comment "Relates a Parliament period to a session."@en ;
	rdfs:domain pt:ParliamentPeriod ;
	rdfs:range pt:Session ;
	rdfs:isDefinedBy <http://parliament.uk/ontologies/time-period/> .
	
pt:hasProrogationPeriod rdf:type owl:ObjectProperty ;
	rdfs:label "hasProrogationPeriod"@en ;
	rdfs:comment "Relates a Parliament period to a prorogation period."@en ;
	rdfs:domain pt:ParliamentPeriod ;
	rdfs:range pt:ProrogationPeriod ;
	rdfs:isDefinedBy <http://parliament.uk/ontologies/time-period/> .

pt:hasTerm rdf:type owl:ObjectProperty ;
	rdfs:label "hasTerm"@en ;
	rdfs:comment "Relates a session to a term."@en ;
	rdfs:domain pt:Session ;
	rdfs:range pt:Term ;
	rdfs:isDefinedBy <http://parliament.uk/ontologies/time-period/> .
	
pt:hasRecess rdf:type owl:ObjectProperty ;
	rdfs:label "hasRecess"@en ;
	rdfs:comment "Relates a session to a recess."@en ;
	rdfs:domain pt:Session ;
	rdfs:range pt:Recess ;
	rdfs:isDefinedBy <http://parliament.uk/ontologies/time-period/> .
	
pt:hasStatutoryDay rdf:type owl:ObjectProperty ;
	rdfs:label "hasStatutoryDay"@en ;
	rdfs:comment "Relates a term to a statutory day."@en ;
	rdfs:domain pt:Term ;
	rdfs:range pt:StatutoryDay ;
	rdfs:isDefinedBy <http://parliament.uk/ontologies/time-period/> .
	
pt:hasRecessStatutoryDay rdf:type owl:ObjectProperty ;
	rdfs:label "hasRecessStatutoryDay"@en ;
	rdfs:comment "Relates a recess to a statutory day."@en ;
	rdfs:domain pt:Recess ;
	rdfs:range pt:StatutoryDay ;
	rdfs:isDefinedBy <http://parliament.uk/ontologies/time-period/> .
	
pt:houseHasTerm rdf:type owl:ObjectProperty ;
	rdfs:label "houseHasTerm"@en ;
	rdfs:comment "Relates a House to a term. Allows for different term periods in different Houses."@en ;
	rdfs:domain pt:House ;
	rdfs:range pt:Term ;
	rdfs:isDefinedBy <http://parliament.uk/ontologies/time-period/> .

pt:houseHasRecess rdf:type owl:ObjectProperty ;
	rdfs:label "houseHasRecess"@en ;
	rdfs:comment "Relates a House to a recess. Allows for different recess periods in different Houses."@en ;
	rdfs:domain pt:House ;
	rdfs:range pt:Recess ;
	rdfs:isDefinedBy <http://parliament.uk/ontologies/time-period/> .
	
pt:hasSittingDay rdf:type owl:ObjectProperty ;
	rdfs:label "hasSittingDay"@en ;
	rdfs:comment "Relates a term to a sitting day."@en ;
	rdfs:domain pt:Term ;
	rdfs:range pt:SittingDay ;
	rdfs:isDefinedBy <http://parliament.uk/ontologies/time-period/> .
	
pt:hasTablingDay rdf:type owl:ObjectProperty ;
	rdfs:label "hasTablingDay"@en ;
	rdfs:comment "Relates a term to a tabling day."@en ;
	rdfs:domain pt:Term ;
	rdfs:range pt:TablingDay ;
	rdfs:isDefinedBy <http://parliament.uk/ontologies/time-period/> .

pt:hasRecessTablingDay rdf:type owl:ObjectProperty ;
	rdfs:label "hasRecessTablingDay"@en ;
	rdfs:comment "Relates a recess to a tabling day. Allows for tabling days to happen in a recess period."@en ;
	rdfs:domain pt:Recess ;
	rdfs:range pt:TablingDay ;
	rdfs:isDefinedBy <http://parliament.uk/ontologies/time-period/> .
	
pt:hasPrintingDay rdf:type owl:ObjectProperty ;
	rdfs:label "hasPrintingDay"@en ;
	rdfs:comment "Relates a term to a printing day."@en ;
	rdfs:domain pt:Term ;
	rdfs:range pt:PrintingDay ;
	rdfs:isDefinedBy <http://parliament.uk/ontologies/time-period/> .

pt:hasRecessPrintingDay rdf:type owl:ObjectProperty ;
	rdfs:label "hasRecessPrintingDay"@en ;
	rdfs:comment "Relates a recess to a printing day. Allows for printing days to happen in a recess period."@en ;
	rdfs:domain pt:Recess ;
	rdfs:range pt:PrintingDay ;
	rdfs:isDefinedBy <http://parliament.uk/ontologies/time-period/> .
	
pt:hasPreElectionDissolutionPeriod rdf:type owl:ObjectProperty ;
	rdfs:label "hasPreElectionDissolutionPeriod"@en ;
	rdfs:comment "Relates a dissolution period to a pre-election dissolution period."@en ;
	rdfs:domain pt:DissolutionPeriod ;
	rdfs:range pt:PreElectionDissolutionPeriod ;
	rdfs:isDefinedBy <http://parliament.uk/ontologies/time-period/> .
	
pt:hasPostElectionDissolutionPeriod rdf:type owl:ObjectProperty ;
	rdfs:label "hasPostElectionDissolutionPeriod"@en ;
	rdfs:comment "Relates a dissolution period to a post-election dissolution period."@en ;
	rdfs:domain pt:DissolutionPeriod ;
	rdfs:range pt:PostElectionDissolutionPeriod ;
	rdfs:isDefinedBy <http://parliament.uk/ontologies/time-period/> .
	
	
	
#######  Data properties ##### 

pt:proposedStartDate rdf:type owl:DatatypeProperty ;
	rdfs:label "proposedStartDate"@en ;
	rdfs:comment "Time period has a proposed start date."@en ;
	rdfs:domain pt:TimePeriod ;
	rdfs:range xsd:date ;
	rdfs:isDefinedBy <http://parliament.uk/ontologies/time-period/> .
	
pt:proposedEndDate rdf:type owl:DatatypeProperty ;
	rdfs:label "proposedEndDate"@en ;
	rdfs:comment "Time period has a proposed end date."@en ;
	rdfs:domain pt:TimePeriod ;
	rdfs:range xsd:date ;
	rdfs:isDefinedBy <http://parliament.uk/ontologies/time-period/> .
	
pt:parliamentNumber rdf:type owl:DatatypeProperty ;
	rdfs:label "parliamentNumber"@en ;
	rdfs:comment "Parliament period has an ordinal number. Numbered from the Act of Union 1800."@en ;
	rdfs:domain pt:ParliamentPeriod ;
	rdfs:range xsd:integer ;
	rdfs:isDefinedBy <http://parliament.uk/ontologies/time-period/> .