@prefix pl: <http://parliament.uk/ontologies/laying/> . 
@prefix xsd: <http://www.w3.org/2001/XMLSchema#> . 
@prefix rdf: <http://www.w3.org/1999/02/22-rdf-syntax-ns#> .
@prefix dcterms: <http://purl.org/dc/terms/> .
@prefix owl:     <http://www.w3.org/2002/07/owl#> .
@prefix rdfs:    <http://www.w3.org/2000/01/rdf-schema#> .
@prefix foaf:	<http://xmlns.com/foaf/0.1/> .

<http://parliament.uk/ontologies/laying/> 
    rdf:type owl:Ontology ;
    dcterms:title "Laying ontology"@en ;
    dcterms:created "2018-02-06"^^xsd:date ;
	dcterms:rights "Open Parliament Licence v3.0"@en ;
    dcterms:description "Laying ontology for UK Parliament, describing the process of laying papers before a House and any subsequent withdrawal."@en;
	foaf:depiction <https://ukparliament.github.io/ontologies/laying/laying.png> ;
	foaf:maker
		[ foaf:name "Robert Brook"; foaf:homepage <https://robert-brook.com/> ],
		[ foaf:name "Stephen McGinness" ],
		[ foaf:name "Michael Smethurst"; foaf:homepage <http://smethur.st/> ],
	    [ foaf:name "Anya Somerville" ].


#######  Classes #####

pl:House rdf:type owl:Class ;
	rdfs:label "House"@en ;
	rdfs:comment "A parliamentary House. For example, the House of Lords."@en ;
	rdfs:isDefinedBy <http://parliament.uk/ontologies/laying/> .

pl:LayingOrWithdrawal rdf:type owl:Class ;
	rdfs:label "Laying or withdrawal"@en ;
	rdfs:comment "The act of laying a paper before a House or withdrawing a paper from a House."@en ;
	rdfs:isDefinedBy <http://parliament.uk/ontologies/laying/> .

pl:Session rdf:type owl:Class ;
	rdfs:label "Session"@en ;
	rdfs:comment "The period during which Parliament is convened. The first session of a parliament begins on the same day as the parliament period: this date is given in the dissolution proclamation at the end of the previous parliament. The session ends on the day set in a subsequent prorogation proclamation. Subsequent sessions within the parliament period begin and end on dates set in subsequent prorogation proclamations. The last session of a parliament ends with prorogation followed by dissolution. Session periods are the same for both Houses."@en ;
	rdfs:isDefinedBy <http://parliament.uk/ontologies/laying/> .
	
pl:LayingBody rdf:type owl:Class ;
	rdfs:label "Laying body"@en ;
	rdfs:comment "A body competent to lay papers before a House or Houses."@en ;
	rdfs:isDefinedBy <http://parliament.uk/ontologies/laying/> .
	
pl:Laying rdf:type owl:Class ;
	rdfs:subClassOf pl:LayingOrWithdrawal ;
	rdfs:label "Laying"@en ;
	rdfs:comment "The act of making available a paper and any supporting documents into a House. Papers may be laid before both Houses on the same day."@en ;
	rdfs:isDefinedBy <http://parliament.uk/ontologies/laying/> .

pl:Withdrawal rdf:type owl:Class ;
	rdfs:subClassOf pl:LayingOrWithdrawal ;
	rdfs:label "Withdrawal"@en ;
	rdfs:comment "The act of withdrawing a paper previously laid before a House."@en ;
	rdfs:isDefinedBy <http://parliament.uk/ontologies/laying/> .

pl:Person rdf:type owl:Class ;
	rdfs:label "Person"@en ;
	rdfs:comment "A person."@en ;
	rdfs:isDefinedBy <http://parliament.uk/ontologies/laying/> .

pl:LayingAuthority rdf:type owl:Class ;
	rdfs:label "Laying authority"@en ;
	rdfs:comment "The authority under which a paper is laid before a House. Legislation may impose a duty on a body to lay papers before a House, these are laid 'by Act'. Command papers are laid in a House by the government and are laid 'by Command'. A paper is laid in the House of Commons or House of Lords either 'by Act' or 'by Command'."@en ;
	rdfs:isDefinedBy <http://parliament.uk/ontologies/laying/> .
	
pl:LayingDuty rdf:type owl:Class ;
	rdfs:label "Laying duty"@en ;
	rdfs:comment "The duty of a body to lay papers before a House as imposed by an Act of Parliament."@en ;
	rdfs:isDefinedBy <http://parliament.uk/ontologies/laying/> .
	
pl:LaidPaper rdf:type owl:Class ;
	rdfs:label "Laid paper"@en ;
	rdfs:comment "A paper having been laid before a House. Papers and supporting documents may be laid as a bundle."@en ;
	rdfs:isDefinedBy <http://parliament.uk/ontologies/laying/> .
	
pl:WithdrawnPaper rdf:type owl:Class ;
	rdfs:label "Withdrawn paper"@en ;
	rdfs:comment "A paper withdrawn after having been laid. Papers or documents forming part of a bundle may be individually withdrawn."@en ;
	rdfs:isDefinedBy <http://parliament.uk/ontologies/laying/> .
	
	

#######  Object properties ##### 

pl:hasHouse rdf:type owl:ObjectProperty ;
	rdfs:label "Has House"@en ;
	rdfs:comment "Relates an act of laying or withdrawing a paper to the House in which the paper is laid or withdrawn."@en ;
	rdfs:domain pl:LayingOrWithdrawal ;
	rdfs:range pl:House ;
	rdfs:isDefinedBy <http://parliament.uk/ontologies/laying/> .
	
pl:hasSession rdf:type owl:ObjectProperty ;
	rdfs:label "Has session"@en ;
	rdfs:comment "Relates an act of laying or withdrawing a paper to the session in which the paper is laid or withdrawn. Papers laid during a prorogation period are considered laid into the session which has been prorogued."@en ;
	rdfs:domain pl:LayingOrWithdrawal ;
	rdfs:range pl:Session ;
	rdfs:isDefinedBy <http://parliament.uk/ontologies/laying/> .
	
pl:hasLayingBody rdf:type owl:ObjectProperty ;
	rdfs:label "Has laying body"@en ;
	rdfs:comment "Relates an act of laying or withdrawal a paper to the laying body laying or withdrawing it."@en ;
	rdfs:domain pl:LayingOrWithdrawal ;
	rdfs:range pl:LayingBody ;
	rdfs:isDefinedBy <http://parliament.uk/ontologies/laying/> .
	
pl:hasLayingPerson rdf:type owl:ObjectProperty ;
	rdfs:label "Has laying person"@en ;
	rdfs:comment "Relates an act of laying a paper to the person laying it."@en ;
	rdfs:domain pl:Laying ;
	rdfs:range pl:Person ;
	rdfs:isDefinedBy <http://parliament.uk/ontologies/laying/> .
	
pl:hasLayingAuthority rdf:type owl:ObjectProperty ;
	rdfs:label "Has laying authority"@en ;
	rdfs:comment "Relates an act of laying a paper to a laying authority."@en ;
	rdfs:domain pl:Laying ;
	rdfs:range pl:LayingAuthority ;
	rdfs:isDefinedBy <http://parliament.uk/ontologies/laying/> .
	
pl:hasLayingDuty rdf:type owl:ObjectProperty ;
	rdfs:label "Has laying duty"@en ;
	rdfs:comment "Relates an act of laying a paper to a duty to lay papers under an Act."@en ;
	rdfs:domain pl:Laying ;
	rdfs:range pl:LayingDuty ;
	rdfs:isDefinedBy <http://parliament.uk/ontologies/laying/> .
	
pl:lays rdf:type owl:ObjectProperty ;
	rdfs:label "Lays"@en ;
	rdfs:comment "Relates an act of laying a paper to the paper which has been laid."@en ;
	rdfs:domain pl:Laying ;
	rdfs:range pl:LaidPaper ;
	rdfs:isDefinedBy <http://parliament.uk/ontologies/laying/> .
	
pl:withdraws rdf:type owl:ObjectProperty ;
	rdfs:label "Withdraws"@en ;
	rdfs:comment "Relates an act of withdrawing a paper to the paper which has been withdrawn."@en ;
	rdfs:domain pl:Withdrawal ;
	rdfs:range pl:WithdrawnPaper ;
	rdfs:isDefinedBy <http://parliament.uk/ontologies/laying/> .	

pl:replaces rdf:type owl:ObjectProperty ;
	rdfs:label "Replaces"@en ;
	rdfs:comment "Relates a laid paper to the withdrawn paper being replaced."@en ;
	rdfs:domain pl:LaidPaper ;
	rdfs:range pl:WithdrawnPaper ;
	rdfs:isDefinedBy <http://parliament.uk/ontologies/laying/> .
				

#######  Data properties ##### 

pl:laidOn rdf:type owl:DatatypeProperty ;
	rdfs:label "Laid on"@en ;
	rdfs:comment "Relates an act of laying a paper to the date on which the laying occurs. This date falls within a parliamentary session or prorogation period, and not during a dissolution period."@en ;
	rdfs:domain pl:Laying ;
	rdfs:range xsd:date ;
	rdfs:isDefinedBy <http://parliament.uk/ontologies/laying/> .
	
pl:withdrawnOn rdf:type owl:DatatypeProperty ;
	rdfs:label "Withdrawn on"@en ;
	rdfs:comment "Relates an act of withdrawal of a paper to the date on which the withdrawal occurs. This date falls within a parliamentary session or prorogation period, and not during a dissolution period."@en ;
	rdfs:domain pl:Withdrawal ;
	rdfs:range xsd:date ;
	rdfs:isDefinedBy <http://parliament.uk/ontologies/laying/> .