@prefix ptr: <http://parliament.uk/ontologies/treaty/> . 
@prefix xsd: <http://www.w3.org/2001/XMLSchema#> . 
@prefix rdf: <http://www.w3.org/1999/02/22-rdf-syntax-ns#> .
@prefix dcterms: <http://purl.org/dc/terms/> .
@prefix owl:     <http://www.w3.org/2002/07/owl#> .
@prefix rdfs:    <http://www.w3.org/2000/01/rdf-schema#> .
@prefix foaf:	<http://xmlns.com/foaf/0.1/> .

<http://parliament.uk/ontologies/treaty/> 
    rdf:type owl:Ontology ;
    dcterms:title "Treaty ontology"@en ;
    dcterms:created "2019-01-16"^^xsd:date ;
	dcterms:rights "Open Parliament Licence v3.0"@en ;
    dcterms:description "An ontology describing the form of treaties considered by UK Parliament."@en ;
	foaf:depiction <https://ukparliament.github.io/ontologies/treaty/treaty.png> ;
	foaf:maker
		[ foaf:name "David Beamish" ],
		[ foaf:name "Robert Brook"; foaf:homepage <https://robert-brook.com/> ],
		[ foaf:name "Jack Dent" ],
		[ foaf:name "Michael Smethurst"; foaf:homepage <http://smethur.st/> ],
	    [ foaf:name "Anya Somerville" ],
		[ foaf:name "Jane White" ] .


#######  Classes ##### 	

ptr:Treaty rdf:type owl:Class ;
	rdfs:label "Treaty"@en ;
	rdfs:comment "A treaty between two or more parties. Treaties between nation states are described by the Vienna Convention on the Law of Treaties. Treaties between nation states and international organisations and between international organisations themselves are described by the Vienna Convention on the Law of Treaties between States and International Organizations or between International Organizations."@en ;
	rdfs:isDefinedBy <http://parliament.uk/ontologies/treaty/> .
	
ptr:NotYetInForceTreaty rdf:type owl:Class ;
	rdfs:subClassOf ptr:Treaty ;
	rdfs:label "Not yet in force treaty"@en ;
	rdfs:comment "A treaty that is not in force in the United Kingdom."@en ;
	rdfs:isDefinedBy <http://parliament.uk/ontologies/treaty/> .
	
ptr:InForceTreaty rdf:type owl:Class ;
	rdfs:subClassOf ptr:Treaty ;
	rdfs:label "In force treaty"@en ;
	rdfs:comment "A treaty that is in force."@en ;
	rdfs:isDefinedBy <http://parliament.uk/ontologies/treaty/> .
	
ptr:NoLongerInForceTreaty rdf:type owl:Class ;
	rdfs:subClassOf ptr:Treaty ;
	rdfs:label "No longer in force treaty"@en ;
	rdfs:comment "A treaty that has previously been in force and is no longer in force. A treaty may include sunset clauses which cause some or all of the treaty to no longer be in force. A treaty may be overtaken by another treaty, either explicitly or implicitly."@en ;
	rdfs:isDefinedBy <http://parliament.uk/ontologies/treaty/> .
	
ptr:Action rdf:type owl:Class ;
	rdfs:label "Action"@en ;
	rdfs:comment "An action by a party on a treaty."@en ;
	rdfs:isDefinedBy <http://parliament.uk/ontologies/treaty/> .

ptr:ActionType rdf:type owl:Class ;
	rdfs:label "Action type"@en ;
	rdfs:comment "The type of action by a party on a treaty. These include signing, ratification, accession or bringing into force."@en ;
	rdfs:isDefinedBy <http://parliament.uk/ontologies/treaty/> .
		
ptr:Party rdf:type owl:Class ;
	rdfs:label "Party"@en ;
	rdfs:comment "An entity with the capacity to enter into treaty obligations."@en ;
	rdfs:isDefinedBy <http://parliament.uk/ontologies/treaty/> .

ptr:State rdf:type owl:Class ;
	rdfs:subClassOf ptr:Party ;
	rdfs:label "State"@en ;
	rdfs:comment "A state."@en ;
	rdfs:isDefinedBy <http://parliament.uk/ontologies/treaty/> .
	
ptr:InternationalOrganisation rdf:type owl:Class ;
	rdfs:subClassOf ptr:Party ;
	rdfs:label "International organisation"@en ;
	rdfs:comment "An organisation with the capacity to enter into treaty obligations, being a supranational body such as the United Nations or an intergovernmental organisation."@en ;
	rdfs:isDefinedBy <http://parliament.uk/ontologies/treaty/> .
	
ptr:TreatySeriesItem rdf:type owl:Class ;
	rdfs:label "Treaty series item"@en ;
	rdfs:comment "A treaty is in one series. Whilst the treaty is not yet in force in the United Kingdom it is in either the bilateral, multilateral or European Union series. If the treaty comes into force it is in the Treaty Series."@en ;
	rdfs:isDefinedBy <http://parliament.uk/ontologies/treaty/> .
	
ptr:TreatySeries rdf:type owl:Class ;
	rdfs:label "Treaty series"@en ;
	rdfs:comment "A series of which a treaty is an item. This is one of the bilateral series, the multilateral series, the European Union series or the Treaty Series. One of the four treaty series is itself called the Treaty Series."@en ;
	rdfs:isDefinedBy <http://parliament.uk/ontologies/treaty/> .
	
ptr:DraftAndMadeStatutoryInstrumentSubjectToParliamentaryProcedure rdf:type owl:Class ;
	rdfs:label "Draft and made statutory instrument subject to parliamentary procedure"@en ;
	rdfs:comment "The National Archives classify made instruments as legislation and draft instruments as draft legislation. Parliament considers both made and draft instruments as part of the legislative process, distinct from a FRBR work as used by The National Archives. Parliament includes draft instruments in its description of statutory instruments which are modelled here together."@en ;
	rdfs:isDefinedBy <http://parliament.uk/ontologies/treaty/> .
	
ptr:Bill rdf:type owl:Class ;
	rdfs:label "Bill"@en ;
	rdfs:comment "A bill presented to Parliament."@en ;
	rdfs:isDefinedBy <http://parliament.uk/ontologies/treaty/> .

ptr:GovernmentOrganisation rdf:type owl:Class ;
	rdfs:label "Government organisation"@en ;
	rdfs:comment "A government department, agency or public body with responsibility for a specific sector of public administration."@en ;
	rdfs:isDefinedBy <http://parliament.uk/ontologies/treaty/> .
	

	
##### Object properties ####

ptr:completesAction rdf:type owl:ObjectProperty ;
	rdfs:label "Completes action"@en ;
	rdfs:comment "Relates a party to an action on a treaty. A party may take many actions on one treaty over time, or on many treaties over time. An action is always by one party."@en ;
	rdfs:domain ptr:Party ;
	rdfs:range ptr:Action ;
	rdfs:isDefinedBy <http://parliament.uk/ontologies/treaty/> .
	
ptr:hasActionType rdf:type owl:ObjectProperty ;
	rdfs:label "Has action type"@en ;
	rdfs:comment "Relates an action to its type."@en ;
	rdfs:domain ptr:Action ;
	rdfs:range ptr:ActionType ;
	rdfs:isDefinedBy <http://parliament.uk/ontologies/treaty/> .
	
ptr:onTreaty rdf:type owl:ObjectProperty ;
	rdfs:label "On treaty"@en ;
	rdfs:comment "Relates an action by a party to a treaty. A treaty may have many actions over time. An action is on a single treaty."@en ;
	rdfs:domain ptr:Action ;
	rdfs:range ptr:Treaty ;
	rdfs:isDefinedBy <http://parliament.uk/ontologies/treaty/> .
	
ptr:asSeriesItem rdf:type owl:ObjectProperty ;
	rdfs:label "As series item"@en ;
	rdfs:comment "Relates a treaty to a treaty series item. A treaty may belong to more than one series by means of a series item. The series will change when the treaty comes into force in the United Kingdom. A series item is formed of a treaty."@en ;
	rdfs:domain ptr:Treaty ;
	rdfs:range ptr:TreatySeriesItem ;
	rdfs:isDefinedBy <http://parliament.uk/ontologies/treaty/> .
	
ptr:inSeries rdf:type owl:ObjectProperty ;
	rdfs:label "In series"@en ;
	rdfs:comment "Relates a treaty series item to a treaty series. A series may have one or more items, or none. A series item places a treaty in a single series."@en ;
	rdfs:domain ptr:TreatySeriesItem ;
	rdfs:range ptr:TreatySeries ;
	rdfs:isDefinedBy <http://parliament.uk/ontologies/treaty/> .
	
ptr:siSatisfies rdf:type owl:ObjectProperty ;
	rdfs:label "SI satisfies"@en ;
	rdfs:comment "Relates a draft or made statutory instrument subject to parliamentary procedure to a treaty which requires the SI to be in force before the treaty can be satisfied."@en ;
	rdfs:domain ptr:DraftAndMadeStatutoryInstrumentSubjectToParliamentaryProcedure ;
	rdfs:range ptr:Treaty ;
	rdfs:isDefinedBy <http://parliament.uk/ontologies/treaty/> .
	
ptr:billSatisfies rdf:type owl:ObjectProperty ;
	rdfs:label "Bill satisfies"@en ;
	rdfs:comment "Relates a bill to a treaty which requires the bill to be in force as an Act before the treaty can be satisfied."@en ;
	rdfs:domain ptr:Bill ;
	rdfs:range ptr:Treaty ;
	rdfs:isDefinedBy <http://parliament.uk/ontologies/treaty/> .
	
ptr:leadDepartment rdf:type owl:ObjectProperty ;
	rdfs:label "Lead department"@en ;
	rdfs:comment ""@en ;
	rdfs:domain ptr:Treaty ;
	rdfs:range ptr:GovernmentOrganisation ;
	rdfs:isDefinedBy <http://parliament.uk/ontologies/treaty/> .
					
	
##### Data properties ####

ptr:occursOn rdf:type owl:DatatypeProperty ;
	rdfs:label "Occurs on"@en ;
	rdfs:comment "The date on which an action was taken or is due to be taken."@en ;
	rdfs:domain ptr:Action ;
	rdfs:range xsd:date ;
	rdfs:isDefinedBy <http://parliament.uk/ontologies/treaty/> .
			
ptr:seriesItemCitation rdf:type owl:DatatypeProperty ;
	rdfs:label "Series item citation"@en ;
	rdfs:comment "Relates a treaty series item to its citation as part of a series."@en ;
	rdfs:domain ptr:TreatySeriesItem ;
	rdfs:range rdfs:Literal ;
	rdfs:isDefinedBy <http://parliament.uk/ontologies/treaty/> .

ptr:commandPaperNumber rdf:type owl:DatatypeProperty ;
	rdfs:label "Command paper number"@en ;
	rdfs:comment ""@en ;
	rdfs:domain ptr:Treaty ;
	rdfs:range rdfs:Literal ;
	rdfs:isDefinedBy <http://parliament.uk/ontologies/treaty/> .

ptr:commandPaperPrefix rdf:type owl:DatatypeProperty ;
	rdfs:label "Command paper prefix"@en ;
	rdfs:comment ""@en ;
	rdfs:domain ptr:Treaty ;
	rdfs:range rdfs:Literal ;
	rdfs:isDefinedBy <http://parliament.uk/ontologies/treaty/> .

ptr:comingIntoForceNote rdf:type owl:DatatypeProperty ;
	rdfs:label "Coming into force note"@en ;
	rdfs:comment "A coming into force note sets out details of the commencement of a treaty."@en ;
	rdfs:domain ptr:Treaty ;
	rdfs:range rdf:langString ;
	rdfs:isDefinedBy <http://parliament.uk/ontologies/treaty/> .
	
ptr:comingIntoForceDate rdf:type owl:DatatypeProperty ;
	rdfs:label "Coming into force date"@en ;
	rdfs:comment "The date on which a treaty comes into force for all parties."@en ;
	rdfs:domain ptr:Treaty ;
	rdfs:range xsd:date ;
	rdfs:isDefinedBy <http://parliament.uk/ontologies/treaty/> .